Nemonuri/Executions/InfiniteExecutionFragment/Basic.lean
@@ -7,6 +7,9 @@ public import Nemonuri.Executions.FiniteExecutionFragment.Raws
 
 namespace Nemonuri.TransitionSystem
 
+open Cslib
+open scoped ωSequence
+
 variable {ts: TransitionSystem}
 
 def IsInfiniteExecutionFragment (raw: ts.InfiniteExecutionFragmentRaw) : Prop := ⦃i: Nat⦄ → (raw.states i) ─⌞(raw.actions i)⌟→{ts} (raw.states (i + 1))
@@ -17,6 +20,24 @@ theorem mk (raw: ts.InfiniteExecutionFragmentRaw) (x: (i: Nat) → (raw.states i
 
 theorem apply {raw} (x: ts.IsInfiniteExecutionFragment raw) (i: Nat) : (raw.states i) ─⌞(raw.actions i)⌟→{ts} (raw.states (i + 1)) := @x i
 
+variable {ef: ts.InfiniteExecutionFragmentRaw}
+
+theorem stepL (h: ts.IsInfiniteExecutionFragment ef) (state0: ts.S) (action0: ts.Act) (req: state0 ─⌞action0⌟→{ts} (ef.states 0))
+  : ts.IsInfiniteExecutionFragment (ef.stepL state0 action0) := by
+  refine .mk _ ?_
+  intro i
+  simp
+  rcases i with _ | ⟨n⟩
+  · simpa using req
+  · simp
+    exact h.apply n
+
+theorem tail (h: ts.IsInfiniteExecutionFragment ef) : ts.IsInfiniteExecutionFragment ef.tail := by
+  refine .mk _ ?_
+  intro i
+  simp [InfiniteExecutionFragmentRaw.tail]
+  exact h.apply (i+1)
+
 end IsInfiniteExecutionFragment
 
 @[defeq]
@@ -24,7 +45,7 @@ theorem isInfiniteExecutionFragment_eq_omegaExecution (raw: ts.InfiniteExecution
   : ts.IsInfiniteExecutionFragment raw = ts.lts.OmegaExecution raw.states raw.actions :=
   rfl
 
-
+@[ext]
 structure InfiniteExecutionFragment (ts: TransitionSystem) where
   raw: ts.InfiniteExecutionFragmentRaw
   is_valid: ts.IsInfiniteExecutionFragment raw
@@ -34,16 +55,13 @@ structure InfiniteExecutionFragment (ts: TransitionSystem) where
 
 namespace InfiniteExecutionFragment
 
-open Cslib
-open scoped ωSequence
-
 variable {ts: TransitionSystem} (ρ: ts.InfiniteExecutionFragment)
 
 def states : ωSequence ts.S := ρ.raw.states
 
 def actions : ωSequence ts.Act := ρ.raw.actions
 
-theorem is_infiniteExecutionFragment : ts.IsInfiniteExecutionFragment ⟨ρ.states, ρ.actions⟩ := ρ.is_valid
+--theorem is_infiniteExecutionFragment : ts.IsInfiniteExecutionFragment ⟨ρ.states, ρ.actions⟩ := ρ.is_valid
 
 def mk' (states: ωSequence ts.S) (actions: ωSequence ts.Act) (req: ts.IsInfiniteExecutionFragment ⟨states, actions⟩) : ts.InfiniteExecutionFragment :=
   ⟨⟨states, actions⟩, req⟩
@@ -55,7 +73,7 @@ theorem mk'_states {states actions req} : (@mk' ts states actions req).states = 
 theorem mk'_actions {states actions req} : (@mk' ts states actions req).actions = actions := rfl
 
 @[defeq, simp]
-theorem mk'_eta : mk' ρ.states ρ.actions ρ.is_infiniteExecutionFragment = ρ := rfl
+theorem mk'_eta : mk' ρ.states ρ.actions ρ.is_valid = ρ := rfl
 
 @[elab_as_elim]
 def indMk'
@@ -65,28 +83,32 @@ def indMk'
         motive (InfiniteExecutionFragment.mk' states actions req))
   (t: ts.InfiniteExecutionFragment)
   : motive t :=
-  mk' t.states t.actions t.is_infiniteExecutionFragment |> Eq.subst t.mk'_eta
+  mk' t.states t.actions t.is_valid |> Eq.subst t.mk'_eta
 
 def state0 := ρ.states 0
 
 def action0 := ρ.actions 0
 
+/-
 theorem tail_preserves_isInfiniteExecutionFragment : ts.IsInfiniteExecutionFragment ⟨ρ.states.tail, ρ.actions.tail⟩ := by
   refine IsInfiniteExecutionFragment.mk _ ?_
   dsimp
   intro i
   exact ρ.is_valid.apply (i+1)
+-/
 
-def tail : ts.InfiniteExecutionFragment :=
-  mk' ρ.states.tail ρ.actions.tail ρ.tail_preserves_isInfiniteExecutionFragment
-
-@[defeq, simp]
-theorem tail_states : ρ.tail.states = ρ.states.tail := by dsimp [tail]
+def tail : ts.InfiniteExecutionFragment := .mk ρ.raw.tail ρ.is_valid.tail
 
 @[defeq, simp]
-theorem tail_actions : ρ.tail.actions = ρ.actions.tail := by dsimp [tail]
+theorem tail_states : ρ.tail.states = ρ.states.tail := by dsimp [tail]; congr
 
+@[defeq, simp]
+theorem tail_actions : ρ.tail.actions = ρ.actions.tail := by dsimp [tail]; congr
 
+@[defeq]
+theorem tail_raw : ρ.tail.raw = ρ.raw.tail := rfl
+
+/-
 theorem stepL_preserves_isInfiniteExecutionFragment {state0: ts.S} {action0: ts.Act} (req: state0 ─⌞action0⌟→{ts} ρ.state0)
   : ts.IsInfiniteExecutionFragment ⟨state0 ::ω ρ.states, action0 ::ω ρ.actions⟩ := by
     refine IsInfiniteExecutionFragment.mk _ ?_
@@ -97,32 +119,64 @@ theorem stepL_preserves_isInfiniteExecutionFragment {state0: ts.S} {action0: ts.
     | succ i ih =>
       simp
       exact ρ.is_valid.apply i
+-/
 
 def stepL (state0: ts.S) (action0: ts.Act) (req: state0 ─⌞action0⌟→{ts} ρ.state0) : ts.InfiniteExecutionFragment :=
-  mk' (state0 ::ω ρ.states) (action0 ::ω ρ.actions) (ρ.stepL_preserves_isInfiniteExecutionFragment req)
+  .mk (ρ.raw.stepL state0 action0) (ρ.is_valid.stepL state0 action0 req)
+
+section StepL
+
+variable {ρ : ts.InfiniteExecutionFragment} (state0: ts.S) (action0: ts.Act) (req: state0 ─⌞action0⌟→{ts} ρ.state0)
 
 @[defeq, simp]
-theorem stepL_tail {tail state0 action0 req} : (@stepL ts tail state0 action0 req).tail = tail := rfl
+theorem stepL_tail : (stepL ρ state0 action0 req).tail = ρ := rfl
 
 @[defeq, simp]
-theorem stepL_state0 {tail state0 action0 req} : (@stepL ts tail state0 action0 req).state0 = state0 := rfl
+theorem stepL_state0 : (stepL ρ state0 action0 req).state0 = state0 := rfl
 
 @[defeq, simp]
-theorem stepL_action0 {tail state0 action0 req} : (@stepL ts tail state0 action0 req).action0 = action0 := rfl
+theorem stepL_action0 : (stepL ρ state0 action0 req).action0 = action0 := rfl
 
-theorem tail_canStepL : ρ.state0 ─⌞ρ.action0⌟→{ts} ρ.tail.state0 := by
-  dsimp
-  have lm1 := @ρ.is_valid 0
-  refine Iff.mp ?_ lm1
-  rw [← propext_iff]
+@[defeq, simp]
+theorem stepL_states : (stepL ρ state0 action0 req).states = state0 ::ω ρ.states := rfl
+
+@[defeq, simp]
+theorem stepL_actions : (stepL ρ state0 action0 req).actions = action0 ::ω ρ.actions := rfl
+
+@[defeq]
+theorem stepL_raw : (stepL ρ state0 action0 req).raw = (ρ.raw.stepL state0 action0) := rfl
+
+theorem tr_state0_action0_tail_state0 : ρ.state0 ─⌞ρ.action0⌟→{ts} ρ.tail.state0 := by
+  dsimp [InfiniteExecutionFragment.state0, InfiniteExecutionFragment.action0]
+  exact ρ.is_valid.apply 0
+
+
+
+end StepL
+
+theorem stepL_eta : (stepL ρ.tail ρ.state0 ρ.action0 ρ.tr_state0_action0_tail_state0) = ρ := by
+  refine InfiniteExecutionFragment.ext ?_
+  dsimp [stepL, tail, state0, action0]
+  exact InfiniteExecutionFragmentRaw.tail_stepL
+
+  --rcases ρ with ⟨raw, lm1⟩
+  --simp [tail_raw, stepL_raw]
+
+/-
+  cases ρ using indMk' with
+  | mk' sts ats lm1 =>
+    dsimp [InfiniteExecutionFragment.stepL, InfiniteExecutionFragment.tail]
+    congr
+-/
+/-
+  dsimp [InfiniteExecutionFragment.stepL, InfiniteExecutionFragment.tail]
   congr
-
-theorem stepL_eta : (stepL ρ.tail ρ.state0 ρ.action0 ρ.tail_canStepL) = ρ := by
-  dsimp [stepL]
-  conv => rhs; rw [← ρ.mk'_eta]
+  dsimp [InfiniteExecutionFragmentRaw.stepL, InfiniteExecutionFragmentRaw.tail]
   congr
-  · dsimp [state0, tail]; simp only [ωSequence.eta]
-  · dsimp [action0, tail]; simp only [ωSequence.eta]
+  · dsimp [InfiniteExecutionFragment.state0, InfiniteExecutionFragment.states]; simp
+  · dsimp [InfiniteExecutionFragment.action0, InfiniteExecutionFragment.actions]; simp
+-/
+
 
 @[elab_as_elim]
 def indStepL
@@ -132,7 +186,7 @@ def indStepL
           motive (InfiniteExecutionFragment.stepL tail state0 action0 req))
   (t: ts.InfiniteExecutionFragment)
   : motive t :=
-  stepL t.tail t.state0 t.action0 t.tail_canStepL |> Eq.subst t.stepL_eta
+  stepL t.tail t.state0 t.action0 t.tr_state0_action0_tail_state0 |> Eq.subst t.stepL_eta
 
 
 
