Nemonuri/Executions/InfiniteExecutionFragment/Raws.lean
@@ -2,6 +2,7 @@ module
 
 public import Nemonuri.TransitionSystem
 public import Nemonuri.Sequence
+public import Nemonuri.Executions.ExecutionEmptyLabel
 
 @[expose] public section
 
@@ -9,18 +10,89 @@ namespace Nemonuri.TransitionSystem
 
 open Cslib
 
+@[ext]
 structure InfiniteExecutionFragmentRaw (ts: TransitionSystem) where
   states : ωSequence ts.S
   actions : ωSequence ts.Act
 
 namespace InfiniteExecutionFragmentRaw
 
-variable {ts: TransitionSystem}
+variable {ts: TransitionSystem} {ef: ts.InfiniteExecutionFragmentRaw}
 
 def ofListRepeat (states: List ts.S) (actions: List ts.Act) (req1: states ≠ []) (req2: actions ≠ []) : ts.InfiniteExecutionFragmentRaw :=
   ⟨.ofListRepeat states req1, .ofListRepeat actions req2⟩
 
 
+def toSeqLabel (_: ts.InfiniteExecutionFragmentRaw) : Sequence.Label := .infinite
+
+def toStatesEmptyLabel (_: ts.InfiniteExecutionFragmentRaw) : ExecutionEmptyLabel .states := .states (.nonempty)
+
+def toActionsEmptyLabel (_: ts.InfiniteExecutionFragmentRaw) : ExecutionEmptyLabel .actions := .actions (.nonempty)
+
+instance : HasLabel Sequence.Label ts.InfiniteExecutionFragmentRaw := ⟨toSeqLabel⟩
+
+instance : HasLabel (ExecutionEmptyLabel .states) ts.InfiniteExecutionFragmentRaw := ⟨toStatesEmptyLabel⟩
+
+instance : HasLabel (ExecutionEmptyLabel .actions) ts.InfiniteExecutionFragmentRaw := ⟨toActionsEmptyLabel⟩
+
+
+
+@[defeq, simp]
+theorem toSeqLabel_eq_infinite : ef.toSeqLabel = .infinite := rfl
+
+@[defeq, simp]
+theorem toStatesEmptyLabel_eq_nonempty : ef.toStatesEmptyLabel = .states (.nonempty) := rfl
+
+@[defeq, simp]
+theorem toActionsEmptyLabel_eq_nonempty : ef.toActionsEmptyLabel = .actions (.nonempty) := rfl
+
+section Mk
+
+variable {sts: ωSequence ts.S} {ats: ωSequence ts.Act}
+
+@[defeq, simp]
+theorem mk_states : (InfiniteExecutionFragmentRaw.mk sts ats).states = sts := rfl
+
+@[defeq, simp]
+theorem mk_actions : (InfiniteExecutionFragmentRaw.mk sts ats).actions = ats := rfl
+
+end Mk
+
+open scoped ωSequence
+
+def stepL (tail: ts.InfiniteExecutionFragmentRaw) (state0: ts.S) (action0: ts.Act) : ts.InfiniteExecutionFragmentRaw :=
+  ⟨state0 ::ω tail.states, action0 ::ω tail.actions⟩
+
+section StepL
+
+variable {tl: ts.InfiniteExecutionFragmentRaw} {s0: ts.S} {a0: ts.Act}
+
+@[defeq, simp]
+theorem stepL_states : (tl.stepL s0 a0).states = s0 ::ω tl.states := rfl
+
+@[defeq, simp]
+theorem stepL_actions : (tl.stepL s0 a0).actions = a0 ::ω tl.actions := rfl
+
+end StepL
+
+
+
+def tail (ef: ts.InfiniteExecutionFragmentRaw) : ts.InfiniteExecutionFragmentRaw := ⟨ef.states.tail, ef.actions.tail⟩
+
+section Tail
+
+variable {s0: ts.S} {a0: ts.Act}
+
+@[defeq, simp]
+theorem stepL_tail : (ef.stepL s0 a0).tail = ef := by
+  cases ef
+  rfl
+
+theorem tail_stepL : (ef.tail.stepL (ef.states 0) (ef.actions 0)) = ef := by
+  dsimp [tail, stepL]
+  simp
+
+end Tail
 
 end InfiniteExecutionFragmentRaw
 
